src/StepM.v
@@ -2,36 +2,46 @@ Require Import Bool List String Peano_dec.
 Require Import Common FMap Syntax Semantics.
 
 Inductive step_m (sys: System): MState -> MLabel -> MState -> Prop :=
-| SmSlt: forall st, step_m sys st emptyRLabel st
-| SmExt: forall pst nst oss orqs oims emsg,
-    fromExternal sys emsg = true ->
-    toInternal sys emsg = true ->
-    pst = {| bst_oss := oss; bst_orqs := orqs; bst_msgs := oims |} ->
+| SmSlt: forall st, step_m sys st (emptyRLabel _) st
+| SmIns: forall pst nst oss orqs msgs eins,
+    eins <> nil ->
+    ValidMsgsExtIn sys eins ->
+    pst = {| bst_oss := oss; bst_orqs := orqs; bst_msgs := msgs |} ->
     nst = {| bst_oss := oss;
              bst_orqs := orqs;
-             bst_msgs := enqMP emsg oims
+             bst_msgs := distributeMsgs eins msgs
           |} ->
-    step_m sys pst (RlblIn emsg) nst
-| SmInt: forall pst nst oss orqs oims oidx os porq pos norq msgs rule outs,
+    step_m sys pst (RlblIns eins) nst
+| SmOuts: forall pst nst oss orqs msgs eouts,
+    eouts <> nil ->
+    Forall (FirstMP msgs) eouts ->
+    ValidMsgsExtOut sys eouts ->
+    pst = {| bst_oss := oss; bst_orqs := orqs; bst_msgs := msgs |} ->
+    nst = {| bst_oss := oss;
+             bst_orqs := orqs;
+             bst_msgs := removeMsgs eouts msgs
+          |} ->
+    step_m sys pst (RlblOuts eouts) nst
+| SmInt: forall pst nst oss orqs msgs oidx os porq pos norq ins rule iouts,
     oidx = rule_oidx rule ->
     In oidx (indicesOf sys) ->
     oss@[oidx] = Some os ->
     orqs@[oidx] = Some porq ->
-    Forall (FirstMP oims) msgs ->
-    ValidMsgsIn oidx msgs ->
-    map (fun tmsg => msg_id tmsg) msgs = rule_mids rule ->
-    In rule (sys_rules sys) ->
-    rule_precond rule os porq msgs ->
-    rule_postcond rule os porq msgs pos norq outs ->
-    ValidMsgOuts oidx outs ->
 
-    pst = {| bst_oss := oss; bst_orqs := orqs; bst_msgs := oims |} ->
+    Forall (FirstMP msgs) ins ->
+    ValidMsgsIn oidx ins ->
+    map (fun tmsg => msg_id tmsg) ins = rule_mids rule ->
+
+    In rule (sys_rules sys) ->
+    rule_precond rule os porq ins ->
+    rule_postcond rule os porq ins pos norq iouts ->
+    ValidMsgsOut oidx iouts ->
+
+    pst = {| bst_oss := oss; bst_orqs := orqs; bst_msgs := msgs |} ->
     nst = {| bst_oss := oss +[ oidx <- pos ];
              bst_orqs := orqs +[ oidx <- norq ];
-             bst_msgs := distributeMsgs
-                           (intOuts sys outs)
-                           (removeMsgs msgs oims)
+             bst_msgs := distributeMsgs iouts (removeMsgs ins msgs)
           |} ->
 
-    step_m sys pst (RlblOuts (Some rule) msgs outs) nst.
+    step_m sys pst (RlblInt (Some rule) ins iouts) nst.
 
